mark-and-sweep/spec/GC.Spec.ChunkedMajorGC.Graph.fsti
@@ -66,6 +66,17 @@ val chunked_major_pointer_classification_preserved
   (mh_final: MH.major_heap)
   : prop
 
+val chunked_major_pointer_classification_preserved_intro
+  (mh_init: MH.major_heap)
+  (mh_final: MH.major_heap)
+  : Lemma
+      (requires
+        (forall (v: U64.t).
+          MarkDefs.chunked_is_pointer_field mh_init v ==
+          MarkDefs.chunked_is_pointer_field mh_final v))
+      (ensures
+        chunked_major_pointer_classification_preserved mh_init mh_final)
+
 val chunked_major_successors_preserved
   (mh_init: MH.major_heap)
   (mh_final: MH.major_heap)
